wip wip wip

core/SerializableUpgradeNet.v
@@ -169,6 +169,222 @@ Section upgrade.
   Qed.
 End upgrade.
 
+Section Serializer.
+  Variable A : Type.
+  Context {sA : Serializer A}.
+  Variable P : A -> Prop.
+
+  Definition lift_strict (b : bytes) : Prop :=
+    match deserialize b with
+    | None => False
+    | Some (a,_) => P a
+    end.
+
+  Definition lift (b : bytes) : Prop :=
+    match deserialize b with
+    | None => True
+    | Some (a,_) => P a
+    end.
+
+  Lemma Serialize_reversible' :
+    forall a, deserialize (serialize a) = Some (a, []).
+  Proof.
+    intros.
+    rewrite <- app_nil_r with (l := serialize a).
+    now rewrite Serialize_reversible.
+  Qed.
+
+  Lemma lift_strict_of_serialize :
+    forall a,
+      P a ->
+      lift_strict (serialize a).
+  Proof.
+    unfold lift_strict.
+    intros.
+    now rewrite Serialize_reversible'.
+  Qed.
+
+  Lemma lift_strict_of_deserialize_some :
+    forall a b rest,
+      deserialize b = Some (a, rest) ->
+      P a ->
+      lift_strict b.
+  Proof.
+    unfold lift_strict.
+    intros.
+    now find_rewrite.
+  Qed.
+
+  Lemma lift_strict_not_None :
+    forall b,
+      deserialize b = None ->
+      lift_strict b ->
+      False.
+  Proof.
+    unfold lift_strict.
+    intros.
+    find_rewrite.
+    auto.
+  Qed.
+
+End Serializer.
+
+Lemma lift_strict_None :
+  forall b1 b2,
+    lift_strict (fun _ => True) b1 <-> lift_strict (fun _ => True) b2 ->
+    deserialize b1 = None ->
+    deserialize b2 = None.
+Proof.
+  unfold lift_strict.
+  intros.
+  repeat break_match; intuition; subst.
+  discriminate.
+Qed.
+
+Section Forall.
+  Variable A : Type.
+  Variable P : A -> Prop.
+
+  Lemma Forall_app_intro :
+    forall xs ys,
+      Forall P xs ->
+      Forall P ys ->
+      Forall P (xs ++ ys).
+  Proof.
+    induction 1; simpl; auto.
+  Qed.
+
+  Lemma Forall_middle_elim :
+    forall xs y zs,
+      Forall P (xs ++ y :: zs) ->
+      Forall P (xs ++ zs).
+  Proof.
+    induction xs; simpl; intros; invc H; eauto.
+  Qed.
+
+  Lemma Forall_middle_elim2 :
+    forall xs y zs,
+      Forall P (xs ++ y :: zs) ->
+      P y.
+  Proof.
+    induction xs; simpl; intros; invc H; eauto.
+  Qed.
+End Forall.
+
+Section TakeStrict.
+
+  Fixpoint take_strict {A} (n : nat) (l : list A) : option (list A) :=
+    match n with
+    | 0 => Some []
+    | S n' => match l with
+             | [] => None
+             | x :: l' => match take_strict n' l' with None => None
+                                                 | Some l'' => Some (x :: l'')
+                         end
+             end
+    end.
+
+  Lemma take_strict_length :
+    forall A n (l : list A) l',
+      take_strict n l = Some l' ->
+      length l' = n.
+  Proof.
+    induction n; simpl; intros.
+    - find_inversion. auto.
+    - repeat break_match; try discriminate.
+      find_inversion. simpl. eauto.
+  Qed.
+
+  Lemma take_strict_lt_None :
+    forall A n (l : list A),
+      length l < n ->
+      take_strict n l = None.
+  Proof.
+    induction n; destruct l; simpl; intros.
+    - omega.
+    - omega.
+    - auto.
+    - now rewrite IHn by omega.
+  Qed.
+
+  Lemma take_strict_unroll :
+    forall A n (l : list A),
+      take_strict (S n) l = match l with
+                            | [] => None
+                            | x :: l' => match take_strict n l' with None => None
+                                                               | Some l'' => Some (x :: l'')
+                                        end
+                            end.
+  Proof. auto. Qed.
+
+  Lemma take_strict_nth_error_Some :
+    forall A n (l : list A) l' a,
+      take_strict n l = Some l' ->
+      nth_error l n = Some a ->
+      take_strict (S n) l = Some (l' ++ [a]).
+  Proof.
+    induction n; intros.
+    - simpl in *. find_inversion. simpl. break_match; congruence.
+    - rewrite take_strict_unroll in *.
+      cbn [nth_error] in *.
+      break_match; try discriminate.
+      break_match_hyp.
+      + find_inversion.
+        erewrite IHn; eauto.
+        auto.
+      + discriminate.
+  Qed.
+
+  Lemma take_strict_length_exact :
+    forall A (l : list A) x,
+      length l = x ->
+      take_strict x l = Some l.
+  Proof.
+    induction l; intros; subst; simpl in *; auto.
+    rewrite IHl; auto.
+  Qed.
+
+  Lemma take_strict_app :
+    forall A (l : list A) x l' l'',
+      take_strict x l = Some l' ->
+      take_strict x (l ++ l'') = Some l'.
+  Proof.
+    induction l; intros; subst; simpl in *; auto.
+    - destruct x; simpl in *; auto. discriminate.
+    - destruct x; simpl in *; auto.
+      break_match_hyp; try discriminate.
+      erewrite IHl; eauto.
+  Qed.
+
+  Lemma take_strict_Prefix :
+    forall A x (l : list A) l',
+      take_strict x l = Some l' ->
+      Prefix l' l.
+  Proof.
+    induction x; intros; simpl in *; auto.
+    - find_inversion. constructor.
+    - repeat break_match; try discriminate.
+      find_inversion.
+      constructor; auto.
+  Qed.
+
+  Lemma take_strict_S_snoc :
+    forall A x (l : list A) l' a,
+      take_strict (S x) l = Some (l' ++ [a]) ->
+      take_strict x l = Some l'.
+  Proof.
+    induction x; intros; rewrite take_strict_unroll in *;
+      destruct l; try discriminate.
+    - destruct l'; auto.
+      destruct l'; discriminate.
+    - break_match_hyp; try discriminate.
+      destruct l'; cbn [app] in *; find_inversion.
+      + find_apply_lem_hyp take_strict_length. cbn [length] in *. omega.
+      + now erewrite IHx by eauto.
+  Qed.
+  
+End TakeStrict.
+      
 
 Module PBKV.
   Inductive name := Primary | Backup.
@@ -322,6 +538,7 @@ Module PBKV.
     Defined.
 
     Definition nop (s : bytes) : bytes * list (name * bytes) * list bytes := (s, [], []).
+    Definition nopm (n : name) (m : bytes) (s : bytes) : bytes * list (name * bytes) * list bytes := (s, [(n, m)], []).
 
     Definition handleInput (n : name) (i : bytes) (s : bytes) :
         bytes * list (name * bytes) * list bytes :=
@@ -355,7 +572,7 @@ Module PBKV.
         bytes * list (name * bytes) * list bytes :=
       match deserialize s with None => nop s
       | Some (s, _) =>
-      match deserialize m with None => nop (serialize s)
+      match deserialize m with None => nopm n m (serialize s)
       | Some (m, _) =>
       match n, m with
       | Primary, Ack =>
@@ -385,77 +602,6 @@ Module PBKV.
     Definition version : Top.version name := Version handleInput handleMsg.
     Definition versions := [(upgrade, version)].
 
-    Section Serializer.
-      Variable A : Type.
-      Context {sA : Serializer A}.
-      Variable P : A -> Prop.
-
-      Definition lift_strict (b : bytes) : Prop :=
-        match deserialize b with
-        | None => False
-        | Some (a,_) => P a
-        end.
-
-      Definition lift (b : bytes) : Prop :=
-        match deserialize b with
-        | None => True
-        | Some (a,_) => P a
-        end.
-
-      Lemma Serialize_reversible' :
-        forall a, deserialize (serialize a) = Some (a, []).
-      Proof.
-        intros.
-        rewrite <- app_nil_r with (l := serialize a).
-        now rewrite Serialize_reversible.
-      Qed.
-
-      Lemma lift_strict_of_serialize :
-        forall a,
-          P a ->
-          lift_strict (serialize a).
-      Proof.
-        unfold lift_strict.
-        intros.
-        now rewrite Serialize_reversible'.
-      Qed.
-
-      Lemma lift_strict_of_deserialize_some :
-        forall a b rest,
-          deserialize b = Some (a, rest) ->
-          P a ->
-          lift_strict b.
-      Proof.
-        unfold lift_strict.
-        intros.
-        now find_rewrite.
-      Qed.
-
-      Lemma lift_strict_not_None :
-        forall b,
-          deserialize b = None ->
-          lift_strict b ->
-          False.
-      Proof.
-        unfold lift_strict.
-        intros.
-        find_rewrite.
-        auto.
-      Qed.
-    End Serializer.
-
-    Lemma lift_strict_None :
-      forall A (sA : Serializer A) b1 b2,
-        lift_strict (fun _ => True) b1 <-> lift_strict (fun _ => True) b2 ->
-        deserialize b1 = None ->
-        deserialize b2 = None.
-    Proof.
-      unfold lift_strict.
-      intros.
-      repeat break_match; intuition; subst.
-      discriminate.
-    Qed.
-
     Lemma nop_no_msgs :
       forall s st ms os,
         nop s = (st, ms, os) -> ms = [].
@@ -471,6 +617,21 @@ Module PBKV.
         nop s = (st, ms, os) -> st = s /\ ms = [] /\ os = [].
     Proof. unfold nop. intuition congruence. Qed.
 
+    Lemma nopm_msgs :
+      forall n m s st ms os,
+        nopm n m s = (st, ms, os) -> ms = [(n, m)].
+    Proof. unfold nopm. congruence. Qed.
+    
+    Lemma nopm_state :
+      forall n m s st ms os,
+        nopm n m s = (st, ms, os) -> st = s.
+    Proof. unfold nopm. congruence. Qed.
+
+    Lemma nopm_elim :
+      forall n m s st ms os,
+        nopm n m s = (st, ms, os) -> st = s /\ ms = [(n, m)] /\ os = [].
+    Proof. unfold nopm. intuition congruence. Qed.
+
 
 
     Lemma only_one_version :
@@ -485,40 +646,19 @@ Module PBKV.
       - destruct n; simpl in *; discriminate.
     Qed.
 
-    Section Forall.
-      Variable A : Type.
-      Variable P : A -> Prop.
-
-      Lemma Forall_app_intro :
-        forall xs ys,
-          Forall P xs ->
-          Forall P ys ->
-          Forall P (xs ++ ys).
-      Proof.
-        induction 1; simpl; auto.
-      Qed.
-
-      Lemma Forall_middle_elim :
-        forall xs y zs,
-          Forall P (xs ++ y :: zs) ->
-          Forall P (xs ++ zs).
-      Proof.
-        induction xs; simpl; intros; invc H; eauto.
-      Qed.
-    End Forall.
-
     Lemma handleMsg_all_packets_deserialize :
       forall h m st st' ms os,
+        lift_strict (fun _ : msg => True) m ->
         handleMsg h m st = (st', ms, os) ->
         Forall (fun p => lift_strict (fun _ : msg => True) (snd p)) ms.
     Proof.
       unfold handleMsg.
       intros.
       repeat break_match;
-          try solve [find_apply_lem_hyp nop_no_msgs; repeat find_rewrite; auto];
-        find_inversion; auto.
-      - constructor; simpl; auto using lift_strict_of_serialize.
-      - constructor; simpl; auto using lift_strict_of_serialize.
+        try solve [find_apply_lem_hyp nop_no_msgs; repeat find_rewrite; auto];
+        try solve [find_inversion; auto; 
+                   constructor; simpl; auto using lift_strict_of_serialize].
+      find_apply_lem_hyp lift_strict_not_None; intuition.
     Qed.
 
     Lemma handleMsg_version :
@@ -561,7 +701,8 @@ Module PBKV.
           * find_apply_lem_hyp only_one_version.
             break_and. subst.
             rewrite handleMsg_version in *.
-            eauto using handleMsg_all_packets_deserialize.
+            eapply handleMsg_all_packets_deserialize; eauto.
+            find_apply_lem_hyp Forall_middle_elim2. simpl in *. auto.
           * eauto using Forall_middle_elim.
         + apply Forall_app_intro.
           * find_apply_lem_hyp only_one_version.
@@ -591,7 +732,9 @@ Module PBKV.
       unfold handleMsg.
       intros.
       repeat break_match; repeat find_inversion;
-      try find_apply_lem_hyp nop_state; subst;
+        try find_apply_lem_hyp nop_state;
+        try find_apply_lem_hyp nopm_state;
+        subst;
       try (rewrite Serialize_reversible' in *; discriminate).
       auto.
     Qed.
@@ -671,29 +814,6 @@ Module PBKV.
       | Some (d, _) => log d
       end.
 
-    Fixpoint take_strict {A} (n : nat) (l : list A) : option (list A) :=
-      match n with
-      | 0 => Some []
-      | S n' => match l with
-               | [] => None
-               | x :: l' => match take_strict n' l' with None => None
-                           | Some l'' => Some (x :: l'')
-                           end
-               end
-      end.
-
-    Lemma take_strict_length :
-      forall A n (l : list A) l',
-        take_strict n l = Some l' ->
-        length l' = n.
-    Proof.
-      induction n; simpl; intros.
-      - find_inversion. auto.
-      - repeat break_match; try discriminate.
-        find_inversion. simpl. eauto.
-    Qed.
-
-
     Definition I (w : world name) : Prop :=
       match deserialize (localState w Primary) with
       | None => packets w = [] /\ get_log (localState w Backup) = []
@@ -717,94 +837,6 @@ Module PBKV.
       get_log [] = get_log (serialize initial_data).
     Proof. auto. Qed.
 
-    Lemma take_strict_lt_None :
-      forall A n (l : list A),
-        length l < n ->
-        take_strict n l = None.
-    Proof.
-      induction n; destruct l; simpl; intros.
-      - omega.
-      - omega.
-      - auto.
-      - now rewrite IHn by omega.
-    Qed.
-
-    Lemma take_strict_unroll :
-      forall A n (l : list A),
-        take_strict (S n) l = match l with
-                              | [] => None
-                              | x :: l' => match take_strict n l' with None => None
-                                          | Some l'' => Some (x :: l'')
-                                          end
-                              end.
-    Proof. auto. Qed.
-
-    Lemma take_strict_nth_error_Some :
-      forall A n (l : list A) l' a,
-        take_strict n l = Some l' ->
-        nth_error l n = Some a ->
-        take_strict (S n) l = Some (l' ++ [a]).
-    Proof.
-      induction n; intros.
-      - simpl in *. find_inversion. simpl. break_match; congruence.
-      - rewrite take_strict_unroll in *.
-        cbn [nth_error] in *.
-        break_match; try discriminate.
-        break_match_hyp.
-        + find_inversion.
-          erewrite IHn; eauto.
-          auto.
-        + discriminate.
-    Qed.
-
-    Lemma take_strict_length_exact :
-      forall A (l : list A) x,
-        length l = x ->
-        take_strict x l = Some l.
-    Proof.
-      induction l; intros; subst; simpl in *; auto.
-      rewrite IHl; auto.
-    Qed.
-
-    Lemma take_strict_app :
-      forall A (l : list A) x l' l'',
-        take_strict x l = Some l' ->
-        take_strict x (l ++ l'') = Some l'.
-    Proof.
-      induction l; intros; subst; simpl in *; auto.
-      - destruct x; simpl in *; auto. discriminate.
-      - destruct x; simpl in *; auto.
-        break_match_hyp; try discriminate.
-        erewrite IHl; eauto.
-    Qed.
-
-    Lemma take_strict_Prefix :
-      forall A x (l : list A) l',
-        take_strict x l = Some l' ->
-        Prefix l' l.
-    Proof.
-      induction x; intros; simpl in *; auto.
-      - find_inversion. constructor.
-      - repeat break_match; try discriminate.
-        find_inversion.
-        constructor; auto.
-    Qed.
-
-    Lemma take_strict_S_snoc :
-      forall A x (l : list A) l' a,
-        take_strict (S x) l = Some (l' ++ [a]) ->
-        take_strict x l = Some l'.
-    Proof.
-      induction x; intros; rewrite take_strict_unroll in *;
-          destruct l; try discriminate.
-      - destruct l'; auto.
-        destruct l'; discriminate.
-      - break_match_hyp; try discriminate.
-        destruct l'; cbn [app] in *; find_inversion.
-        + find_apply_lem_hyp take_strict_length. cbn [length] in *. omega.
-        + now erewrite IHx by eauto.
-    Qed.
-    
     Local Arguments nth_error : simpl never.
     Local Arguments take_strict : simpl never.
     Lemma get_log_serialize :
@@ -1010,7 +1042,7 @@ Module PBKV.
       | Some (ver, rest) =>
         match ver with
         | 0 =>
-          match deserialize rest with
+          match deserialize bs with
           | Some (VersionOne.Put k v, rest) =>
             Some (Put k v, rest)
           | Some (VersionOne.Get k, rest) =>
@@ -1169,6 +1201,7 @@ Module PBKV.
     Defined.
 
     Definition nop (s : bytes) : bytes * list (name * bytes) * list bytes := (s, [], []).
+    Definition nopm (n : name) (m : bytes) (s : bytes) : bytes * list (name * bytes) * list bytes := (s, [(n, m)], []).
 
     Definition handleInput (n : name) (i : bytes) (s : bytes) :
         bytes * list (name * bytes) * list bytes :=
@@ -1206,7 +1239,7 @@ Module PBKV.
         bytes * list (name * bytes) * list bytes :=
       match deserialize s with None => nop s
       | Some (s, _) =>
-      match deserialize m with None => nop (serialize s)
+      match deserialize m with None => nopm n m (serialize s)
       | Some (m, _) =>
       match n, m with
       | Primary, Ack =>
@@ -1247,5 +1280,830 @@ Module PBKV.
 
     Definition version : Top.version name := Version handleInput handleMsg.
     Definition versions := VersionOne.versions ++ [(upgrade, version)].
+
+
+    Lemma nop_no_msgs :
+      forall s st ms os,
+        nop s = (st, ms, os) -> ms = [].
+    Proof. unfold nop. congruence. Qed.
+
+    Lemma nop_state :
+      forall s st ms os,
+        nop s = (st, ms, os) -> st = s.
+    Proof. unfold nop. congruence. Qed.
+
+    Lemma nop_elim :
+      forall s st ms os,
+        nop s = (st, ms, os) -> st = s /\ ms = [] /\ os = [].
+    Proof. unfold nop. intuition congruence. Qed.
+
+    Lemma nopm_msgs :
+      forall n m s st ms os,
+        nopm n m s = (st, ms, os) -> ms = [(n, m)].
+    Proof. unfold nopm. congruence. Qed.
+    
+    Lemma nopm_state :
+      forall n m s st ms os,
+        nopm n m s = (st, ms, os) -> st = s.
+    Proof. unfold nopm. congruence. Qed.
+
+    Lemma nopm_elim :
+      forall n m s st ms os,
+        nopm n m s = (st, ms, os) -> st = s /\ ms = [(n, m)] /\ os = [].
+    Proof. unfold nopm. intuition congruence. Qed.
+
+
+
+    Lemma only_two_versions :
+      forall n u v,
+        nth_error versions n = Some (u, v) ->
+        (u = VersionOne.upgrade /\ v = VersionOne.version /\ n = 0) \/
+        (u = upgrade /\ v = version /\ n = 1).
+    Proof.
+      unfold versions.
+      intros.
+      destruct n; simpl in *.
+      - find_inversion. auto.
+      - destruct n; simpl in *; try find_inversion; auto.
+        destruct n; simpl in *; discriminate.
+    Qed.
+
+    Lemma handleMsg_all_packets_deserialize :
+      forall h m st st' ms os,
+        lift_strict (fun _ : msg => True) m ->
+        handleMsg h m st = (st', ms, os) ->
+        Forall (fun p => lift_strict (fun _ : msg => True) (snd p)) ms.
+    Proof.
+      unfold handleMsg.
+      intros.
+      repeat break_match;
+        try solve [find_apply_lem_hyp nop_no_msgs; repeat find_rewrite; auto];
+        try solve [find_inversion; auto; 
+                   constructor; simpl; auto using lift_strict_of_serialize].
+      find_apply_lem_hyp lift_strict_not_None; intuition.
+    Qed.
+
+    Definition upgrade_msg (m : VersionOne.msg) : msg :=
+      match m with
+      | VersionOne.Cmd i => Cmd (upgrade_input i)
+      | VersionOne.Ack => Ack
+      end.
+
+    Lemma V1V2_input_deserialize :
+      forall b i rest,
+        deserialize b = Some (i, rest) ->
+        deserialize b = Some (upgrade_input i, rest).
+    Proof.
+      intros.
+      unfold deserialize; simpl in *.
+      unfold input_deserialize. break_match.
+      - break_let. subst.
+        repeat find_rewrite.
+        break_match.
+        + break_match; subst; simpl; auto.
+        + exfalso.
+          unfold deserialize in H.
+          simpl in *.
+          unfold VersionOne.input_deserialize in *.
+          repeat find_rewrite.
+          break_if; discriminate.
+      - exfalso.
+        unfold deserialize in H.
+          simpl in *.
+          unfold VersionOne.input_deserialize in *.
+          repeat find_rewrite. discriminate.
+    Qed.
+    
+    Lemma V1V2_list_input_deserialize':
+      forall (n : nat) (l : list VersionOne.input) (rest : list bool) (l' : list bool),
+        list_deserialize_rec VersionOne.input VersionOne.input_Serializer n l' =
+        Some (l, rest) ->
+        list_deserialize_rec input input_Serializer n l' = Some (map upgrade_input l, rest).
+    Proof.
+      induction n; intros; simpl in *; auto.
+      - now find_inversion.
+      - break_match_hyp; try discriminate.
+        break_let. subst. 
+        erewrite V1V2_input_deserialize; eauto.
+        break_match_hyp; try discriminate.
+        break_let. find_inversion.
+        simpl.
+        erewrite IHn; eauto.
+    Qed.
+
+        
+    Lemma V1V2_list_input_deserialize :
+      forall l b rest,
+        deserialize b = Some (l, rest) ->
+        deserialize b = Some (map upgrade_input l, rest).
+    Proof.
+      intros.
+      unfold deserialize in *. simpl in *.
+      unfold list_deserialize in *. simpl in *.
+      break_match; try discriminate.
+      break_let. subst.
+      eauto using V1V2_list_input_deserialize'.
+    Qed.
+    
+    Lemma V1V2_input_serialize :
+      forall i,
+        @deserialize input _ (serialize i) = deserialize (serialize (upgrade_input i)).
+    Proof.
+      intros.
+      rewrite Serialize_reversible'.
+      apply V1V2_input_deserialize.
+      rewrite Serialize_reversible'. auto.
+    Qed.
+
+    Lemma V1V2_msg_deserialize :
+      forall m b rest,
+        deserialize b = Some (m, rest) ->
+        deserialize b = Some (upgrade_msg m, rest).
+    Proof.
+      intros.
+      unfold deserialize in *; simpl in *.
+      unfold msg_deserialize, VersionOne.msg_deserialize in *; simpl in *.
+      break_match; try discriminate.
+      break_let. subst.
+      break_match; try discriminate.
+      break_let. repeat break_if; try discriminate.
+      - break_match_hyp; try discriminate.
+        break_let. subst.
+        find_apply_lem_hyp V1V2_input_deserialize.
+        find_rewrite.
+        now find_inversion.
+      - now find_inversion.
+    Qed.
+    
+    Lemma V1V2_msg_serialize :
+      forall m,
+        @deserialize msg _ (serialize m) = deserialize (serialize (upgrade_msg m)).
+    Proof.
+      intros.
+      rewrite Serialize_reversible'.
+      destruct m; simpl; auto.
+      unfold serialize; simpl; unfold VersionOne.msg_serialize.
+      simpl.
+      unfold deserialize. simpl.
+      unfold msg_deserialize.
+      simpl.
+      rewrite V1V2_input_serialize.
+      rewrite Serialize_reversible'. auto.
+    Qed.
+
+    Lemma V1V2_data_deserialize :
+      forall d b rest,
+        deserialize b = Some (d, rest) ->
+        deserialize b = Some (upgrade_data d, rest).
+    Proof.
+      intros.
+      unfold deserialize in *. simpl in *.
+      unfold data_deserialize, VersionOne.data_deserialize in *.
+      break_match; try discriminate.
+      break_let. subst.
+      break_match_hyp; try discriminate.
+      break_let. subst.
+      erewrite V1V2_list_input_deserialize; eauto.
+      break_match; try discriminate.
+      break_let. now find_inversion.
+    Qed.
+    
+    Lemma V1V2_data_serialize :
+      forall d,
+        @deserialize data _ (serialize d) = deserialize (serialize (upgrade_data d)).
+    Proof.
+      intros.
+      rewrite Serialize_reversible'.
+      apply V1V2_data_deserialize.
+      apply Serialize_reversible'.
+    Qed.
+    
+    Lemma old_handleMsg_all_packets_deserialize :
+      forall h m st st' ms os,
+        lift_strict (fun _ : msg => True) m ->
+        VersionOne.handleMsg h m st = (st', ms, os) ->
+        Forall (fun p => lift_strict (fun _ : msg => True) (snd p)) ms.
+    Proof.
+      unfold VersionOne.handleMsg.
+      intros.
+      repeat break_match;
+        try solve [find_apply_lem_hyp nop_no_msgs; repeat find_rewrite; auto];
+        try solve [find_inversion; auto; 
+                   constructor; simpl; auto using lift_strict_of_serialize].
+      - find_inversion.
+        constructor; auto.
+        simpl. eapply lift_strict_of_deserialize_some; eauto.
+        rewrite V1V2_msg_serialize.
+        rewrite Serialize_reversible'; eauto.
+      - find_inversion.
+        constructor; auto.
+        simpl. eapply lift_strict_of_deserialize_some; eauto.
+        rewrite V1V2_msg_serialize.
+        rewrite Serialize_reversible'; eauto.
+      - find_apply_lem_hyp nopm_msgs.
+        subst. constructor; auto.
+    Qed.
+    
+    Lemma handleMsg_version :
+      Top.handleMsg version = handleMsg.
+    Proof.
+      reflexivity.
+    Qed.
+
+    Lemma handleInput_version :
+      Top.handleInput version = handleInput.
+    Proof.
+      reflexivity.
+    Qed.
+
+    Lemma handleInput_all_packets_deserialize :
+      forall h i st st' ms os,
+        handleInput h i st = (st', ms, os) ->
+        Forall (fun p => lift_strict (fun _ : msg => True) (snd p)) ms.
+    Proof.
+      unfold handleInput.
+      intros.
+      intros.
+      repeat break_match;
+          try solve [find_apply_lem_hyp nop_no_msgs; repeat find_rewrite; auto];
+        find_inversion; auto.
+      constructor; simpl; auto using lift_strict_of_serialize.
+    Qed.
+
+
+    Lemma old_handleInput_all_packets_deserialize :
+      forall h i st st' ms os,
+        VersionOne.handleInput h i st = (st', ms, os) ->
+        Forall (fun p => lift_strict (fun _ : msg => True) (snd p)) ms.
+    Proof.
+      unfold VersionOne.handleInput.
+      intros.
+      intros.
+      repeat break_match;
+        try solve [find_apply_lem_hyp nop_no_msgs; repeat find_rewrite; auto].
+      find_inversion; auto.
+      constructor; simpl; auto.
+      simpl.
+      eapply lift_strict_of_deserialize_some; eauto.
+      rewrite V1V2_msg_serialize.
+      rewrite Serialize_reversible'; eauto.
+    Qed.
+    
+    Lemma all_packets_deserialize :
+      forall w,
+        step_reachable versions w ->
+        Forall (fun p => lift_strict (fun _ : msg => True) (snd p)) (packets w).
+    Proof.
+      induction 1; intros.
+      - unfold initial_world in *. simpl in *. constructor.
+      - clear H0. invcs H.
+        + auto.
+        + repeat find_rewrite.
+          apply Forall_app_intro.
+          * find_apply_lem_hyp only_two_versions. break_or_hyp.
+            -- break_and. subst.
+               rewrite VersionOne.handleMsg_version in *.
+               eapply old_handleMsg_all_packets_deserialize; eauto.
+               find_apply_lem_hyp Forall_middle_elim2. simpl in *. auto.
+            -- break_and. subst.
+               rewrite handleMsg_version in *.
+               eapply handleMsg_all_packets_deserialize; eauto.
+               find_apply_lem_hyp Forall_middle_elim2. simpl in *. auto.
+          * eauto using Forall_middle_elim.
+        + apply Forall_app_intro.
+          * find_apply_lem_hyp only_two_versions. break_or_hyp.
+            -- break_and. subst.
+               rewrite VersionOne.handleInput_version in *.
+               eapply old_handleInput_all_packets_deserialize; eauto.
+            -- break_and. subst.
+               rewrite handleInput_version in *.
+               eapply handleInput_all_packets_deserialize; eauto.
+          * eauto using Forall_middle_elim.
+    Qed.
+
+    Lemma upgrade_deserializes :
+      forall st st',
+        upgrade st = Some st' ->
+        lift_strict (fun _ => True) st'.
+    Proof.
+      unfold upgrade.
+      intros.
+      repeat break_match; try discriminate.
+      find_inversion.
+      auto using lift_strict_of_serialize.
+    Qed.
+
+    Lemma handleMsg_deserializes_None_eq :
+      forall h m st st' ms os,
+        handleMsg h m st = (st', ms, os) ->
+        deserialize st' = None ->
+        st' = st.
+    Proof.
+      unfold handleMsg.
+      intros.
+      repeat break_match; repeat find_inversion;
+        try find_apply_lem_hyp nop_state;
+        try find_apply_lem_hyp nopm_state;
+        subst;
+      try (rewrite Serialize_reversible' in *; discriminate).
+      auto.
+    Qed.
+
+    Lemma handleInput_deserializes_None_eq :
+      forall h m st st' ms os,
+        handleInput h m st = (st', ms, os) ->
+        deserialize st' = None ->
+        st' = st.
+    Proof.
+      unfold handleInput.
+      intros.
+      repeat break_match; repeat find_inversion;
+      try find_apply_lem_hyp nop_state; subst;
+      try (rewrite Serialize_reversible' in *; discriminate).
+      auto.
+    Qed.
+
+    Ltac update_rewrite := rewrite ?@update_same in *; rewrite ?@update_neq in * by congruence.
+
+    Lemma initialized_state_deserializes_v1 :
+      forall w,
+        step_reachable versions w ->
+        (forall h,
+            @deserialize VersionOne.data _ (localState w h) = None  ->
+            nextVersion w h = 0 \/ nextVersion w h = 2).
+    Proof.
+      induction 1; intros.
+      - simpl. auto.
+      - clear H0. invcs H; find_apply_lem_hyp only_two_versions; break_or_hyp; break_and; subst.
+        + destruct (eq_dec h0 h); subst; update_rewrite.
+          * unfold VersionOne.upgrade in *.
+            find_inversion.
+            find_rewrite_lem Serialize_reversible'. discriminate.
+          * find_apply_hyp_hyp.
+            auto.
+        + repeat find_rewrite.
+          destruct (eq_dec h0 h); subst; update_rewrite; auto.
+        + rewrite VersionOne.handleMsg_version in *.
+          destruct (eq_dec h h0); subst; update_rewrite; auto.
+          find_apply_lem_hyp VersionOne.handleMsg_deserializes_None_eq; subst; auto.
+        + destruct (eq_dec h h0); subst; update_rewrite; auto.
+        + rewrite VersionOne.handleInput_version in *.
+          destruct (eq_dec h h0); subst; update_rewrite; auto.
+          find_apply_lem_hyp VersionOne.handleInput_deserializes_None_eq; subst; auto.
+        + destruct (eq_dec h0 h); subst; update_rewrite; auto.
+    Qed.
+
+    Lemma initialized_state_deserializes_v2 :
+      forall w,
+        step_reachable versions w ->
+        (forall h,
+            @deserialize data _ (localState w h) = None  ->
+            nextVersion w h = 0 \/ nextVersion w h = 1).
+    Proof.
+      induction 1; intros.
+      - simpl. auto.
+      - clear H0. invcs H; find_apply_lem_hyp only_two_versions; break_or_hyp; break_and; subst.
+        + destruct (eq_dec h0 h); subst; update_rewrite; try omega.
+          find_apply_hyp_hyp.
+          auto.
+        + repeat find_rewrite.
+          destruct (eq_dec h0 h); subst; update_rewrite; auto.
+          exfalso.
+          unfold upgrade in *.
+          repeat break_match; simpl in *; auto; try congruence.
+          find_inversion.
+          rewrite Serialize_reversible' in *. congruence.
+        + destruct (eq_dec h h0); subst; update_rewrite; auto.
+        + destruct (eq_dec h h0); subst; update_rewrite; auto.
+          find_apply_lem_hyp handleMsg_deserializes_None_eq; subst; auto.
+        + destruct (eq_dec h0 h); subst; update_rewrite; auto.
+        + rewrite handleInput_version in *.
+          destruct (eq_dec h h0); subst; update_rewrite; auto.
+          find_apply_lem_hyp handleInput_deserializes_None_eq; subst; auto.
+    Qed.
+    
+    Lemma version_0_is_init :
+      forall w,
+        step_reachable versions w ->
+        (forall h,
+            nextVersion w h = 0 -> localState w h = []).
+    Proof.
+      induction 1; intros.
+      - auto.
+      - clear H0. invcs H; find_apply_lem_hyp only_two_versions; break_or_hyp; break_and; subst.
+        + destruct (eq_dec h h0); subst; update_rewrite; try discriminate.
+          auto.
+        + destruct (eq_dec h h0); subst; update_rewrite; try discriminate.
+          auto.
+        + assert (h <> h0) by congruence.
+          update_rewrite. auto.
+        + assert (h <> h0) by congruence.
+          update_rewrite. auto.
+        + destruct (eq_dec h h0); subst; update_rewrite; try congruence.
+          auto.
+        + destruct (eq_dec h h0); subst; update_rewrite; try congruence.
+          auto.
+    Qed.
+
+    Definition backup_prefix (w : world name) : Prop :=
+      match deserialize (localState w Backup) with
+      | None => True
+      | Some (backup, _) =>
+      match deserialize (localState w Primary) with
+      | None => True
+      | Some (primary, _) =>
+      Prefix (log backup) (log primary)
+      end
+      end.
+
+    Definition get_log (b : bytes) : list input :=
+      match deserialize b with
+      | None => []
+      | Some (d, _) => log d
+      end.
+
+    Definition lift_packets : list (name * bytes) -> list (name * option (msg * bytes)) :=
+      map (fun x => (fst x, deserialize (snd x))).
+
+    Definition I (w : world name) : Prop :=
+      match deserialize (localState w Primary) with
+      | None => packets w = [] /\ get_log (localState w Backup) = []
+      | Some (primary, _) =>
+        (packets w = [] /\
+         take_strict (nextIndex primary) (log primary) = Some (get_log (localState w Backup))) \/
+        (exists i, lift_packets (packets w) = [(Backup, Some (Cmd i, []))] /\
+              take_strict (S (nextIndex primary)) (log primary) =
+                  Some (get_log (localState w Backup) ++ [i])) \/
+        (lift_packets (packets w) = [(Primary, Some (Ack, []))] /\
+         take_strict (S (nextIndex primary)) (log primary) = Some (get_log (localState w Backup)))
+      end.
+
+    Lemma deserialize_data_nil :
+      deserialize [] = @None (data * _).
+    Proof.
+      auto.
+    Qed.
+
+    Lemma get_log_initialize :
+      get_log [] = get_log (serialize VersionOne.initial_data).
+    Proof. auto. Qed.
+
+    Local Arguments nth_error : simpl never.
+    Local Arguments take_strict : simpl never.
+    Lemma get_log_serialize :
+      forall x,
+        get_log (serialize x) = log x.
+    Proof.
+      intros.
+      unfold get_log.
+      rewrite Serialize_reversible'; auto.
+    Qed.
+
+    Lemma get_log_serialize_V1V2 :
+      forall x : VersionOne.data,
+        get_log (serialize x) = log (upgrade_data x).
+    Proof.
+      intros.
+      unfold get_log.
+      rewrite V1V2_data_serialize.
+      rewrite Serialize_reversible'; auto.
+    Qed.
+    
+    Lemma map_single :
+      forall A B l (f : A -> B) b,
+        map f l = [b] ->
+        exists a,
+          f a = b /\ l = [a].
+    Proof.
+      intros.
+      destruct l; simpl in *; try congruence.
+      find_inversion.
+      find_apply_lem_hyp map_eq_nil; subst.
+      eauto.
+    Qed.
+      
+    Lemma I_packet_to_primary_elim :
+      forall w mb, I w ->
+              In (Primary, mb) (packets w) ->
+              deserialize mb = Some (Ack, []) /\
+              packets w = [(Primary, mb)] /\
+              exists primary rest,
+                deserialize (localState w Primary) = Some (primary, rest) /\
+                take_strict (S (nextIndex primary)) (log primary) =
+                Some (get_log (localState w Backup)).
+    Proof.
+      unfold I.
+      intros.
+      repeat break_match; repeat break_or_hyp; break_exists; break_and; subst;
+        repeat find_rewrite; simpl in *; repeat break_or_hyp; intuition.
+      - unfold lift_packets in *.
+        find_apply_lem_hyp map_single.
+        break_exists. intuition. repeat find_rewrite.
+        simpl in *. intuition. subst. simpl in *. congruence.
+      - unfold lift_packets in *.
+        find_apply_lem_hyp map_single.
+        break_exists. intuition. repeat find_rewrite.
+        simpl in *. intuition. subst. simpl in *. congruence.
+      - unfold lift_packets in *.
+        find_apply_lem_hyp map_single.
+        break_exists. intuition. repeat find_rewrite.
+        simpl in *. intuition. subst. simpl in *. congruence.
+      - unfold lift_packets in *.
+        find_apply_lem_hyp map_single.
+        break_exists. intuition. repeat find_rewrite.
+        simpl in *. intuition. subst. simpl in *. congruence.
+      - unfold lift_packets in *.
+        find_apply_lem_hyp map_single.
+        break_exists. intuition. repeat find_rewrite.
+        simpl in *. intuition. subst. simpl in *. auto.
+      - eauto.
+    Qed.
+
+    Lemma I_packet_to_backup_elim :
+      forall w mb, I w ->
+              In (Backup, mb) (packets w) ->
+              (exists i, deserialize mb = Some (Cmd i, []) /\
+                    packets w = [(Backup, mb)] /\
+                    exists primary rest,
+                      deserialize (localState w Primary) = Some (primary, rest) /\
+                      take_strict (S (nextIndex primary)) (log primary) =
+                      Some (get_log (localState w Backup) ++ [i])).
+    Proof.
+      unfold I.
+      intros.
+      repeat break_match; repeat break_or_hyp; break_exists; break_and; subst;
+        repeat find_rewrite; simpl in *; repeat break_or_hyp; intuition.
+      - unfold lift_packets in *.
+        find_apply_lem_hyp map_single.
+        break_exists. intuition. repeat find_rewrite.
+        simpl in *. intuition. subst. simpl in *.
+        find_inversion. eauto 10.
+      - unfold lift_packets in *.
+        find_apply_lem_hyp map_single.
+        break_exists. intuition. repeat find_rewrite.
+        simpl in *. intuition. subst. simpl in *. congruence.
+    Qed.
+
+    Lemma get_log_deserialize_Some :
+      forall s d rest,
+        deserialize s = Some (d, rest) ->
+        get_log s = log d.
+    Proof.
+      unfold get_log.
+      intros.
+      now find_rewrite.
+    Qed.
+
+    Lemma upgrade_msg_Ack :
+      forall m,
+        upgrade_msg m = Ack ->
+        m = VersionOne.Ack.
+    Proof.
+      destruct m; simpl in *; congruence.
+    Qed.
+
+    Definition lower_input (i : input) : option VersionOne.input :=
+      match i with
+      | Put k v => Some (VersionOne.Put k v)
+      | Get k => Some (VersionOne.Get k)
+      | _ => None
+      end.
+
+    Lemma upgrade_msg_Cmd :
+      forall m i,
+        upgrade_msg m = Cmd i ->
+        exists j,
+          upgrade_input j = i /\
+          m = VersionOne.Cmd j.
+    Proof.
+      intros.
+      destruct m; simpl in *; try congruence.
+      find_inversion. eauto.
+    Qed.
+
+    Lemma upgrade_data_length_log :
+      forall d,
+        length (VersionOne.log d) =
+        length (log (upgrade_data d)).
+    Proof.
+      intros. unfold upgrade_data.
+      simpl.
+      now rewrite map_length.
+    Qed.
+    
+    Lemma upgrade_data_nextIndex :
+      forall d,
+        VersionOne.nextIndex d = nextIndex (upgrade_data d).
+    Proof.
+      now destruct d.
+    Qed.
+
+    Lemma I_true :
+      forall w,
+        step_reachable versions w ->
+        I w.
+    Proof.
+      induction 1 using step_reachable_ind.
+      - unfold I, initial_world. simpl. auto.
+      - invcs H0.
+        + (* upgrade case *)
+          find_apply_lem_hyp only_two_versions. break_or_hyp.
+          * {
+              break_and. subst.
+              unfold I in *. simpl in *.
+              unfold VersionOne.upgrade in *. find_inversion.
+              destruct h; subst; update_rewrite.
+              * (* Primary *)
+                rewrite V1V2_data_serialize.
+                rewrite Serialize_reversible'.
+                simpl in *.
+                rewrite version_0_is_init in * by auto.
+                rewrite deserialize_data_nil in *.
+                unfold take_strict.
+                intuition congruence.
+              * (* Backup *)
+                rewrite version_0_is_init with (h := Backup) in * by auto.
+                now rewrite get_log_initialize in *.
+            }
+          * {
+              break_and. subst.
+              unfold I in *. simpl in *.
+              unfold upgrade in *. break_match_hyp; try congruence.
+              break_let. find_inversion.
+              destruct h; subst; update_rewrite.
+              * (* Primary *)
+                rewrite Serialize_reversible'.
+                repeat find_rewrite.
+                find_apply_lem_hyp V1V2_data_deserialize.
+                now find_rewrite.
+              * (* Backup *)
+                find_apply_lem_hyp V1V2_data_deserialize.
+                erewrite get_log_deserialize_Some in IHstep_reachable; eauto.
+                erewrite get_log_deserialize_Some; eauto using Serialize_reversible'.
+            }
+        + (* msg case *)
+          find_apply_lem_hyp only_two_versions. break_or_hyp. {
+          break_and. subst.
+          rewrite VersionOne.handleMsg_version in *.
+          unfold VersionOne.handleMsg in *. simpl in *.
+          break_match_hyp; [| find_apply_lem_hyp initialized_state_deserializes_v1;
+                              eauto; omega].
+          break_let. subst.
+          break_match_hyp.
+          * break_let. subst.
+            break_match_hyp; subst; update_rewrite.
+            -- (* Primary *)
+              find_eapply_lem_hyp I_packet_to_primary_elim; [|repeat find_rewrite; eauto with *].
+              break_and. break_exists. break_and.
+              find_apply_lem_hyp V1V2_msg_deserialize.
+              repeat find_rewrite.
+              find_inversion.
+              find_apply_lem_hyp upgrade_msg_Ack.
+              subst.
+              unfold I. simpl. update_rewrite.
+              destruct xs; [|destruct xs; discriminate].
+              cbn [app] in *. find_inversion.
+              find_apply_lem_hyp V1V2_data_deserialize.
+              repeat find_rewrite.
+              find_inversion.
+              break_match_hyp.
+              ++ break_let. find_inversion.
+                 rewrite V1V2_data_serialize.
+                 rewrite Serialize_reversible'. simpl in *.
+                 rewrite app_nil_r.
+                 break_match; auto.
+                 simpl in *. 
+                 rewrite V1V2_msg_serialize.
+                 rewrite Serialize_reversible'. simpl.
+                 intuition eauto using take_strict_nth_error_Some, map_nth_error.
+              ++ find_apply_lem_hyp nop_elim. break_and. subst.
+                 exfalso.
+                 find_apply_lem_hyp nth_error_None.
+                 rewrite upgrade_data_length_log in *.
+                 rewrite upgrade_data_nextIndex in *.
+                 rewrite take_strict_lt_None in * by omega.
+                 discriminate.
+            -- (* Backup *)
+              find_eapply_lem_hyp I_packet_to_backup_elim; [|eauto with *].
+              break_exists. break_and. break_exists. break_and.
+              find_apply_lem_hyp V1V2_msg_deserialize.
+              find_apply_lem_hyp V1V2_data_deserialize.
+              repeat find_rewrite. repeat find_inversion.
+              find_apply_lem_hyp upgrade_msg_Cmd.
+              break_exists. break_and.
+              subst.
+              break_let. find_inversion.
+              destruct xs; [|destruct xs; discriminate].
+              cbn [app] in *. find_inversion.
+              unfold I. simpl. update_rewrite. repeat find_rewrite.
+              right. right.
+              rewrite V1V2_msg_serialize. simpl.
+              rewrite Serialize_reversible'. intuition.
+              rewrite get_log_serialize_V1V2.
+              erewrite get_log_deserialize_Some by eauto.
+              simpl.
+              now rewrite map_app. 
+          * find_apply_lem_hyp nopm_elim. intuition. subst.
+            simpl. rewrite app_nil_r.
+            Lemma get_log_deserialize :
+              forall b1 b2,
+                deserialize b1 = deserialize b2 ->
+                get_log b1 = get_log b2.
+            Proof.
+              intros. unfold get_log.
+              repeat find_rewrite.
+              break_match; auto.
+            Qed.
+
+            Lemma I_equiv :
+              forall w w',
+                I w ->
+                (forall h, deserialize (localState w' h) = deserialize (localState w h)) ->
+                PEr
+                I w'.
+            Proof.
+              intros.
+              unfold I in *.
+              break_match; repeat find_higher_order_rewrite; auto;
+                repeat erewrite get_log_deserialize by eauto; auto.
+            Qed.
+
+            eapply state_deserialize; eauto.
+            
+           
+            find_apply_lem_hyp all_packets_deserialize.
+            exfalso.
+            find_eapply_lem_hyp Forall_forall; [|eauto with *].
+            simpl in *.
+            unfold lift_strict in *.
+            break_match_hyp; intuition.
+            
+            eapply lift_strict_not_None with (A := msg); eauto.
+          }
+        + (* handleInput *)
+          find_apply_lem_hyp only_one_version.
+          break_and. subst.
+          rewrite handleInput_version in *.
+          unfold I, handleInput in *. simpl in *.
+          break_match_hyp; [| find_apply_lem_hyp initialized_state_deserializes; auto; omega].
+          break_let. subst.
+          break_match_hyp.
+          * break_let. break_match_hyp; subst.
+            -- repeat find_rewrite.
+               update_rewrite.
+               find_inversion.
+               rewrite Serialize_reversible'. simpl.
+               break_if; simpl.
+               ++ right. left.
+                  intuition.
+                  ** repeat find_rewrite. eexists; intuition eauto.
+                     rewrite take_strict_length_exact in *; auto; [congruence|].
+                     rewrite app_length. simpl. omega.
+                  ** exfalso.
+                     break_exists. break_and.
+                     erewrite take_strict_lt_None in *; try discriminate. omega.
+                  ** exfalso. erewrite take_strict_lt_None in *; try discriminate. omega.
+               ++ repeat break_or_hyp.
+                  ** left.
+                     break_and.
+                     erewrite take_strict_app; eauto.
+                  ** right. left.
+                     break_exists; break_and.
+                     erewrite take_strict_app; eauto.
+                  ** right. right.
+                     break_and.
+                     erewrite take_strict_app; eauto.
+            -- find_apply_lem_hyp nop_elim.
+               break_and; subst. simpl in *.
+               update_rewrite.
+               unfold get_log in *.
+               repeat find_rewrite.
+               rewrite Serialize_reversible'. auto.
+          * find_apply_lem_hyp nop_elim.
+            break_and; subst. simpl in *.
+            destruct h; update_rewrite; repeat find_rewrite;
+              try rewrite Serialize_reversible'; auto.
+            unfold get_log in *.
+            repeat find_rewrite.
+            rewrite Serialize_reversible'. auto.
+    Qed.
+
+
+    Theorem backup_prefix_true :
+      forall w,
+        step_reachable versions w ->
+        backup_prefix w.
+    Proof.
+      intros.
+      find_apply_lem_hyp I_true.
+      unfold I, backup_prefix in *.
+      repeat break_match; auto.
+      unfold get_log in *. repeat find_rewrite.
+      intuition eauto using take_strict_Prefix.
+      - break_exists. intuition.
+        find_apply_lem_hyp take_strict_S_snoc.
+        eauto using take_strict_Prefix.
+    Qed.
+    
   End VersionTwo.
 End PBKV.
